\documentclass{unswmaths}
\usepackage{color}
\begin{document}
\author{Adam J. Gray}
\studentno{3329798}
\subject{Number Theory}
\title{Assignment}

\unswtitle

\section*{Question 1}
Write $ \omega(n) $ for the number of (distinct) prime divisors of $ n $, 
$ \Omega(n) $ for the number of prime factors of $ n $, counted with 
repetition. Thus if, $ n = \prod_{j=1}^m p_j^{k_j} $, then $ \omega(n) = m $,
and $ \Omega(n) = \sum_{j=1}^{m} k_j $.
\subsubsection*{Part a}
Prove that $ 2^{\omega(n)} \leq \tau(n) \leq 2^{\Omega(n)} \leq n $ for 
$ n \geq 2 $.
\subsubsection*{Part b}
When does $ \tau(n) = 2^{\omega(n)} $.

\hrulefill

\subsection*{\textcolor{blue}{Solution}}
\subsubsection*{\textcolor{blue}{Part a}}
Firstly we prove that $ 2^\omega(n) \leq \tau(n) $. 
From the lecture notes we have that if $ n = \prod_{j=1}^m p_j^{k_j} $
then $ \tau(n) = \prod^{m}_{j=1}(k_j + 1) $ so we can say
\begin{align}
	\tau(n) 	&= \prod^{m}_{j=1}\underbrace{(k_j + 1)}_{\geq 2} \nonumber \\
				\label{ineq:qn1a}
				&\leq \prod^{m}_{j=1} 2 \\
				&= 2^m \nonumber \\
				&= 2^{\omega(n)} \nonumber
\end{align}
so $ 2^{\omega(n)} \leq \tau(n) $.

We now show that $ \tau(n) \leq 2^{\Omega(n)} $.
See that 
\begin{align*}
	2^{\Omega(n)} 	&= 2^{\sum_{j=1}^{m} k_j} \\
					&= \prod_{j=1}^{m}2^{k_j}
\end{align*}
and because for all $ k_j \geq 1 $, $ k_j + 1 \leq 2^{k_j} $.
then
\begin{align*}
	\prod_{j=1}^{m}2^{k_j}	\geq \prod_{j=1}^{m} (k_j + 1) \\
\end{align*}
and thus 
$$
	\tau(n) \leq 2^{\Omega(n)}.
$$
It remains to show that $ 2^{\Omega(n)} \leq n $.
Because we have that $$ n = \prod_{j=1}^m p_j^{k_j} $$ and $$ 2^{\Omega(n)} = \prod_{j=1}^{m}2^{k_j} $$
then it is clear because $ 2 \leq k_j $ for all $ j $. 

So we have shown that $ 2^{\omega(n)} \leq \tau(n) \leq 2^{\Omega(n)} \leq n $.

\hrulefill

\section*{Question 2}
Define the \textbf{Jordan totient function} by 
$$
    n^k\prod_{p|n}(1-p^-k),
$$
where, as usual, the product is taken over the primes. This is a generalization of Euler's
totient function.
\subsubsection*{Part a}
Prove that $ J $ is multiplicative.
\subsubsection*{Part b}
Show that $ J_k(n) = \sum_{d|n} \mu(d) (\frac{n}{d})^k. $
\subsubsection*{Part c}
Find a simple expression (as a product over primes) for $ J^{-1}(n) $.

\hrulefill
\subsection*{\textcolor{blue}{Solution}}
\subsubsection*{\textcolor{blue}{Part a}}
For $ (n,m) = 1 $ see that
$$
    J_k(nm) = (nm)^k \prod_{p|nm} (1-p^{-k})
$$
but as $ (n,m) = 1 $ then $ p | n $ or $ p | m $ but not both so
\begin{align*}
    J_k(nm) &= n^k m^k \prod_{p|n} (1-p^{-k})\prod_{p|m} (1-p^{-k}) \\
        &= \left( n^k \prod{p|n}(1-p^{-k}) \right)\left( n^k \prod{q|m}(1-q^{-k}) \right) \\
        &= J_k(n) J_k(m)
\end{align*}
\qed

\subsubsection*{\textcolor{blue}{Part b}}
Let $ p $ be a prime and observe that
$$
    J_k(p^\alpha) = p^{\alpha k }(1- p^{-k})
$$
and note in addition that $ J_k(1) = 1 $.
Now define 
$$
    \gamma_k(n) := \sum_{d|n} J_k(d) 
$$
and note that since $ J_k $ is multiplicative, so is $ \gamma_k $.

Therefor it we only need to see consider $ \gamma_k(p^\alpha) $, where $ p $ is prime,
to characterize $ \gamma_k $.

Therefore observe that
\begin{align*}
    \gamma_k(p^\alpha) &= \sum_{j = 0}^\alpha J_k(p^\alpha) \\
        &= \sum_{j = 1}^\alpha p^{jk}(1-p^k) + 1 \\
        &= (1-p^{-k}) \sum_{j=1}^\alpha p^{jk} + 1 \\
        &= ( 1 - p^{-k})\left( \frac{p^k - p^{k(\alpha + 1)}}{1 - p^k} \right) + 1 \\
        &= p^{\alpha k}.
\end{align*}
So if $ n = p_1^{\alpha_1} \ldots p_r^{\alpha_r} $ then
\begin{align*}
    \gamma_k(n) &= \gamma_k(p_1^{\alpha_1}) \ldots \gamma_k(p_r^{\alpha_r}) \\
        &= p_1^{\alpha_1 k} \ldots p_r^{\alpha_r k} \\
        &= n^k.
\end{align*}
So we have that
\begin{align*}
    \sum_{d|n} J_k(d) &= n^k
\end{align*}
and hence by Mobius inversion
\begin{align*}
    J_k(d) &= \sum_{d|n} \mu(d) \left(\frac{n}{d}\right)^k.
\end{align*}
\qed
\subsubsection*{\textcolor{blue}{Part c}}

Let $ N^k(n) = n^k $. It is clear that $ N^k $ is completely multiplicative. 
Also see that $ J_k = \mu * N^k $. So by the result in the notes, since $ N^k $ is 
completely multiplicative $ J_k^{-1} = N^{k} $.
\qed

\hrulefill

\section*{Question 3}

Write $ M_2(x) = \sum{ n \leq x } (\mu(n))^2 $.

Hence $ M_2(x) $ counts the number of square free integers $ \leq x $.

\subsubsection*{Part a}
Explain why $ (\mu(n))^2 = \sum_{m^2 | n} \mu(m) $.

\subsubsection*{Part b}
Proce that $ M_2(x) = x \sum_{m \leq \sqrt{x}} \frac{\mu(n)}{m^2} - \sum_{m \leq \sqrt{x}} \mu(m) \left\{ \frac{x}{m^2} \right\} $.

\subsubsection*{Part c}
Deduce that 
$$
	M_2(x) = \frac{6}{\pi^2}x + O(\sqrt{x}).
$$

\subsubsection*{Part d}
Interpret this result in terms of the proportion of square-free numbers
in the interval $[ 1, x] $.
\subsubsection*{Part e}
Use MAPLE (or otherwise) to count the number of square-free numbers between $ 1 $ and $ 1000 $. (Comment!)

\hrulefill

\subsection*{\textcolor{blue}{Solution}}

\subsubsection*{\textcolor{blue}{Part a}}


\end{document}

